\section*{Problem 10}
	\begin{proof}
		Proof by induction. Let the given statement be $P(j = r)$. Consider $P(j = 1)$. Then
		\begin{align*}
			\sum\limits_{k=0}^{1} {_{n + k}\mathrm{C}_{k}} &= {_{n}\mathrm{C}_{0}} + {_{n + 1}\mathrm{C}_{1}}\\
			&= {_{n + 1}\mathrm{C}_{0}} + {_{n + 1}\mathrm{C}_{1}}\\
			&= {_{n + 2}\mathrm{C}_{1}}
		\end{align*}
		by the \textit{Pascal\textquotesingle s rule}: $\left[{_{n}\mathrm{C}_{r}} + {_{n}\mathrm{C}_{r + 1}} = {_{n + 1}\mathrm{C}_{r + 1}}\right]$. Therefore, $P(j = 1)$ is true.\\
		Suppose $P(j = r)$ is true, consider $P(j = r + 1)$.
		\begin{align*}
			\sum\limits_{k=0}^{r + 1} {_{n + k}\mathrm{C}_{k}} &= \sum\limits_{k=0}^{r} {_{n + k}\mathrm{C}_{k}} + {_{n + r + 1}\mathrm{C}_{r + 1}}\\
			&= {_{n + r + 1}\mathrm{C}_{r}} + {_{n + r + 1}\mathrm{C}_{r + 1}}\\
			&= {_{n + r + 2}\mathrm{C}_{r + 1}}
		\end{align*}
		Therefore, $P(j = r + 1)$ is true.\\
	\end{proof}