\section*{Problem 4}
	\begin{proof}
		Note that the definition of NOR is `not OR', i.e.
		\begin{equation*}
			x\downarrow y = \neg(x\vee y)
		\end{equation*}
		First, claim that NOT is expressed by only NOR.
		\begin{align*}
			\neg p=
			\begin{cases}
				0 & \mbox{if }p=1 \\
				1 & \mbox{if }p=0
			\end{cases} =
			\begin{cases}
				p\downarrow p & \mbox{if }p=1 \\
				p\downarrow p & \mbox{if }p=0
			\end{cases}
			= p\downarrow p
		\end{align*}
		Next, claim that OR is expressed by only NOR.
		\begin{align*}
			p\vee q &= \neg\neg(p\vee q) = \neg(\neg(p\vee q))\\
			&= \neg(p\downarrow q) = (p\downarrow q)\downarrow(p\downarrow q)
		\end{align*}
		Therefore, since \{OR, NOT\} is functionally complete, \{NOR\} is functionally complete.\\
	\end{proof}