\section*{Problem 3}
	\begin{proof}
		Let $F$ be DNF of $f$. Then $F = m_1\vee m_2\vee\cdots\vee m_k$, where $m_k$ is conjunctive form. Since $\neg m_k$ is disjunctive form and $\neg\vee = \wedge$, $\neg F$ is CNF.\\
		The CNF form of the above problem is
		\begin{equation*}
			f(w,x,y,z)=\begin{multlined}[t]
				(\neg w\vee\neg x\vee\neg y\vee z)\wedge(\neg w\vee\neg x\vee y\vee z)\wedge(\neg w\vee x\vee \neg y\vee\neg z)\\
				\wedge(\neg w\vee x\vee\neg y\vee z)\wedge(\neg w\vee x\vee y\vee z)\wedge(w\vee\neg x\vee\neg y\vee z)\wedge(w\vee\neg x\vee y\vee\neg z)\\
				\wedge(w\vee\neg x\vee y\vee z)\wedge(w\vee x\vee\neg y\vee z)\wedge(w\vee x\vee y\vee\neg z)\wedge(w\vee x\vee y\vee z)
			\end{multlined}
		\end{equation*}
	\end{proof}